# Kinetic Energy
---
Consider [[Newton's Equation of Motion]]:
$$m\underline{\ddot{r}} = \underline{F}$$
We multiply both sides by $\underline{\dot{r}}$ to get:
$$\begin{aligned} m\underline{\ddot{r}} = \underline{F} &\Rightarrow  m\underline{\dot{r}} \cdot \underline{\ddot{r}} =\underline{\dot{r}}\cdot \underline{F} \\ \\
&\Rightarrow m\frac{d}{dt}\Big(\frac{1}{2}\underline{\dot{r}} \cdot\underline{\dot{r}}\ \Big)=\underline{F} \cdot{\underline{r}} \\ \\
&\Rightarrow \frac{1}{2} m\Big(\underbrace{m\frac{1}{2}\mid\underline{r}^{2} \mid}_{\text{Kinetic Energy } K}\Big)= \underline{F}\cdot \underline{r}\end{aligned}$$
```ad-Definition
Title: **Kinetic Energy**

Kinetic Energy is defined as
$$K = \frac{1}{2}m\mid\underline{v}\mid^{2} = \frac{1}{2}\mid\underline{\dot{r}}\mid^{2}$$
```

*Note:* The second implication came from the [[Chain Rule for Differentiation]]

# Backlinks
---
- [[Energy]]
- [[Newtonian Mechanics]]